add subst for cvterms

Common/Term.lean
@@ -18,24 +18,33 @@ deriving BEq
 
 inductive CvTerm : Type where
 | sym : CvTerm -> CvTerm
-| ax : CvTerm
-| var : CvTerm
-| pi : CvTerm -> CvTerm -> CvTerm
-| lam_mt : CvTerm -> CvTerm -> CvTerm
-| lam_mf : CvTerm -> CvTerm
+| none : CvTerm
+| const : CvTerm
+| bound : Nat -> CvTerm
+| all_congr : CvTerm -> CvTerm -> CvTerm
+| lam_congr : CvTerm -> CvTerm -> CvTerm
 | lam_eta : CvTerm -> CvTerm
-| lam_m0 : CvTerm -> CvTerm
-| app : CvTerm -> CvTerm -> CvTerm
+| lam_mf_erased : CvTerm -> CvTerm
+| lam_m0_erased : CvTerm -> CvTerm
+| app_congr : CvTerm -> CvTerm -> CvTerm
 | app_beta : CvTerm -> CvTerm
-| app_m0 : CvTerm -> CvTerm
-| prod : CvTerm -> CvTerm -> CvTerm
-| pair : CvTerm -> CvTerm
-| fst : CvTerm -> CvTerm
-| snd : CvTerm -> CvTerm
-| eq : CvTerm -> CvTerm -> CvTerm -> CvTerm
-| refl : CvTerm -> CvTerm
-| subst : CvTerm -> CvTerm
-| conv : CvTerm -> CvTerm
+| app_m0_erased : CvTerm -> CvTerm
+| prod_congr : CvTerm -> CvTerm -> CvTerm
+| pair_congr : CvTerm -> CvTerm -> CvTerm -> CvTerm
+| pair_erased : CvTerm -> CvTerm
+| fst_congr : CvTerm -> CvTerm
+| fst_erased : CvTerm -> CvTerm
+| snd_congr : CvTerm -> CvTerm
+| snd_erased : CvTerm -> CvTerm
+| phi_congr : CvTerm -> CvTerm -> CvTerm -> CvTerm
+| phi_erased : CvTerm -> CvTerm
+| eq_congr : CvTerm -> CvTerm -> CvTerm -> CvTerm
+| refl_congr : CvTerm -> CvTerm
+| refl_erased : CvTerm -> CvTerm
+| subst_congr : CvTerm -> CvTerm -> CvTerm
+| subst_erased : CvTerm -> CvTerm
+| conv_congr : CvTerm -> CvTerm -> CvTerm -> CvTerm
+| conv_erased : CvTerm -> CvTerm
 deriving BEq
 
 inductive Term : Type where
@@ -59,38 +68,45 @@ deriving BEq
 notation "★" => Term.const Const.type
 notation "□" => Term.const Const.kind
 
-instance : Inhabited Term where
+instance instInhabitedTerm : Inhabited Term where
   default := Term.none
 
 namespace Term
 
   -- templates
-  -- | i, bound k => sorry
+  -- | i, bound c k => sorry
   -- | i, none => sorry
-  -- | i, type => sorry
-  -- | i, kind => sorry
-  -- | i, lam t1 t2 => sorry
-  -- | i, app t1 t2 => sorry
-  -- | i, all t1 t2 => sorry
-  -- | i, pair t1 t2 => sorry
+  -- | i, const k => sorry
+  -- | i, lam m t1 t2 => sorry
+  -- | i, app m t1 t2 => sorry
+  -- | i, all m t1 t2 => sorry
+  -- | i, pair t1 t2 t3 => sorry
   -- | i, fst t => sorry
   -- | i, snd t => sorry
   -- | i, prod t1 t2 => sorry
+  -- | i, refl t => sorry
+  -- | i, subst t1 t2 => sorry
+  -- | i, phi t1 t2 t3 => sorry
   -- | i, eq t1 t2 t3 => sorry
-  -- | i, int t1 t2 => sorry
-  -- case bound => sorry
-  -- case none => sorry
-  -- case type => sorry
-  -- case kind => sorry
-  -- case lam t1 t2 ih1 ih2 => sorry
-  -- case app t1 t2 ih1 ih2 => sorry
-  -- case all t1 t2 ih1 ih2 => sorry
-  -- case pair t1 t2 ih1 ih2 => sorry
-  -- case fst t ih => sorry
-  -- case snd t ih => sorry
-  -- case prod t1 t2 ih1 ih2 => sorry
-  -- case eq t1 t2 t3 ih1 ih2 ih3 => sorry
-  -- case int t1 t2 ih1 ih2 => sorry
+  -- | i, conv t1 t2 c => sorry
+
+  @[simp]
+  def cvrefl : Term -> CvTerm
+  | bound _ k => .bound k
+  | none => .none
+  | const _ => .const
+  | lam _ t1 t2 => .lam_congr (cvrefl t1) (cvrefl t2)
+  | app _ t1 t2 => .app_congr (cvrefl t1) (cvrefl t2)
+  | all _ t1 t2 => .all_congr (cvrefl t1) (cvrefl t2)
+  | pair t1 t2 t3 => .pair_congr (cvrefl t1) (cvrefl t2) (cvrefl t3)
+  | fst t => .fst_congr (cvrefl t)
+  | snd t => .snd_congr (cvrefl t)
+  | prod t1 t2 => .prod_congr (cvrefl t1) (cvrefl t2)
+  | refl t => .refl_congr (cvrefl t)
+  | subst t1 t2 => .subst_congr (cvrefl t1) (cvrefl t2)
+  | phi t1 t2 t3 => .phi_congr (cvrefl t1) (cvrefl t2) (cvrefl t3)
+  | eq t1 t2 t3 => .eq_congr (cvrefl t1) (cvrefl t2) (cvrefl t3)
+  | conv t1 t2 c => .conv_congr (cvrefl t1) (cvrefl t2) c
 
   @[simp]
   def size : Term -> Nat
