Common/Term/Substitution.lean
@@ -3,17 +3,24 @@ import Common.Term
 namespace Term
   def Ren : Type := Nat -> Nat
 
-  inductive SubstAction : Type where
-  | rename : Nat -> SubstAction
-  | replace : Term -> SubstAction
+  inductive SubstAction (T : Type) : Type where
+  | rename : Nat -> SubstAction T
+  | replace : T -> SubstAction T
 
   namespace SubstAction
-    def size : SubstAction -> Nat
+    def size : SubstAction Term -> Nat
     | .rename _ => 0
     | .replace t => Term.size t
   end SubstAction
 
-  def Subst : Type := Nat -> SubstAction
+  def Subst (T : Type) : Type := Nat -> SubstAction T
+
+  def subst_term_to_subst_cvterm : Subst Term -> Subst CvTerm
+  | σ, n => match σ n with
+    | .rename k => .rename k
+    | .replace t => .replace (cvrefl t)
+
+  prefix:max "▸" => subst_term_to_subst_cvterm
 
   @[simp] def I : Ren := λ n => n
   @[simp] def S : Ren := λ n => n + 1
@@ -24,6 +31,37 @@ namespace Term
     def lift : Ren -> Ren
     | _, 0 => 0
     | σ, n + 1 => σ n + 1
+
+    @[simp]
+    def cvapply : Ren -> CvTerm -> CvTerm
+    | σ, .sym t => .sym (cvapply σ t)
+    | _, .none => .none
+    | _, .const => .const
+    | σ, .bound k => .bound (σ k)
+    | σ, .all_congr t1 t2 => .all_congr (cvapply σ t1) (cvapply (lift σ) t2)
+    | σ, .lam_congr t1 t2 => .lam_congr (cvapply σ t1) (cvapply (lift σ) t2)
+    | σ, .lam_eta t => .lam_eta (cvapply σ t)
+    | σ, .lam_mf_erased t => .lam_mf_erased (cvapply (lift σ) t)
+    | σ, .lam_m0_erased t => .lam_m0_erased (cvapply (lift σ) t)
+    | σ, .app_congr t1 t2 => .app_congr (cvapply σ t1) (cvapply σ t2)
+    | σ, .app_beta t => .app_beta (cvapply σ t)
+    | σ, .app_m0_erased t => .app_m0_erased (cvapply σ t)
+    | σ, .prod_congr t1 t2 => .prod_congr (cvapply σ t1) (cvapply (lift σ) t2)
+    | σ, .pair_congr t1 t2 t3 => .pair_congr (cvapply σ t1) (cvapply σ t2) (cvapply σ t3)
+    | σ, .pair_erased t => .pair_erased (cvapply σ t)
+    | σ, .fst_congr t => .fst_congr (cvapply σ t)
+    | σ, .fst_erased t => .fst_erased (cvapply σ t)
+    | σ, .snd_congr t => .snd_congr (cvapply σ t)
+    | σ, .snd_erased t => .snd_erased (cvapply σ t)
+    | σ, .phi_congr t1 t2 t3 => .phi_congr (cvapply σ t1) (cvapply σ t2) (cvapply σ t3)
+    | σ, .phi_erased t => .phi_erased (cvapply σ t)
+    | σ, .eq_congr t1 t2 t3 => .eq_congr (cvapply σ t1) (cvapply σ t2) (cvapply σ t3)
+    | σ, .refl_congr t => .refl_congr (cvapply σ t)
+    | σ, .refl_erased t => .refl_erased (cvapply σ t)
+    | σ, .subst_congr t1 t2 => .subst_congr (cvapply σ t1) (cvapply σ t2)
+    | σ, .subst_erased t => .subst_erased (cvapply σ t)
+    | σ, .conv_congr t1 t2 t3 => .conv_congr (cvapply σ t1) (cvapply σ t2) (cvapply σ t3)
+    | σ, .conv_erased t => .conv_erased (cvapply σ t)
 
     @[simp]
     def apply : Ren -> Term -> Term
@@ -41,25 +79,65 @@ namespace Term
     | σ, subst t1 t2 => subst (apply σ t1) (apply σ t2)
     | σ, phi t1 t2 t3 => phi (apply σ t1) (apply σ t2) (apply σ t3)
     | σ, eq t1 t2 t3 => eq (apply σ t1) (apply σ t2) (apply σ t3)
-    | σ, conv t1 t2 c => conv (apply σ t1) (apply σ t2) c
+    | σ, conv t1 t2 c => conv (apply σ t1) (apply σ t2) (cvapply σ c)
   end Ren
 
   namespace Subst
-    def from_ren : Ren -> Subst
+    def from_ren : Ren -> Subst T
     | σ, n => .rename (σ n)
 
-    def cons : SubstAction -> Subst -> Subst
+    def cons : SubstAction T -> Subst T -> Subst T
     | t, _, 0 => t
     | _, σ, n + 1 => σ n
 
-    def lift : Subst -> Subst
+    def cvlift : Subst CvTerm -> Subst CvTerm
+    | _, 0 => .rename 0
+    | σ, n + 1 => match (σ n) with
+      | .replace t => .replace (Ren.cvapply S t)
+      | .rename k => .rename (S k)
+
+    def lift : Subst Term -> Subst Term
     | _, 0 => .rename 0
     | σ, n + 1 => match (σ n) with
       | .replace t => .replace (Ren.apply S t)
       | .rename k => .rename (S k)
 
     @[simp]
-    def apply : Subst -> Term -> Term
+    def cvapply : Subst CvTerm -> CvTerm -> CvTerm
+    | σ, .sym t => .sym (cvapply σ t)
+    | _, .none => .none
+    | _, .const => .const
+    | σ, .bound k =>
+      match σ k with
+      | .replace t => t
+      | .rename n => .bound n
+    | σ, .all_congr t1 t2 => .all_congr (cvapply σ t1) (cvapply (cvlift σ) t2)
+    | σ, .lam_congr t1 t2 => .lam_congr (cvapply σ t1) (cvapply (cvlift σ) t2)
+    | σ, .lam_eta t => .lam_eta (cvapply σ t)
+    | σ, .lam_mf_erased t => .lam_mf_erased (cvapply (cvlift σ) t)
+    | σ, .lam_m0_erased t => .lam_m0_erased (cvapply (cvlift σ) t)
+    | σ, .app_congr t1 t2 => .app_congr (cvapply σ t1) (cvapply σ t2)
+    | σ, .app_beta t => .app_beta (cvapply σ t)
+    | σ, .app_m0_erased t => .app_m0_erased (cvapply σ t)
+    | σ, .prod_congr t1 t2 => .prod_congr (cvapply σ t1) (cvapply (cvlift σ) t2)
+    | σ, .pair_congr t1 t2 t3 => .pair_congr (cvapply σ t1) (cvapply σ t2) (cvapply σ t3)
+    | σ, .pair_erased t => .pair_erased (cvapply σ t)
+    | σ, .fst_congr t => .fst_congr (cvapply σ t)
+    | σ, .fst_erased t => .fst_erased (cvapply σ t)
+    | σ, .snd_congr t => .snd_congr (cvapply σ t)
+    | σ, .snd_erased t => .snd_erased (cvapply σ t)
+    | σ, .phi_congr t1 t2 t3 => .phi_congr (cvapply σ t1) (cvapply σ t2) (cvapply σ t3)
+    | σ, .phi_erased t => .phi_erased (cvapply σ t)
+    | σ, .eq_congr t1 t2 t3 => .eq_congr (cvapply σ t1) (cvapply σ t2) (cvapply σ t3)
+    | σ, .refl_congr t => .refl_congr (cvapply σ t)
+    | σ, .refl_erased t => .refl_erased (cvapply σ t)
+    | σ, .subst_congr t1 t2 => .subst_congr (cvapply σ t1) (cvapply σ t2)
+    | σ, .subst_erased t => .subst_erased (cvapply σ t)
+    | σ, .conv_congr t1 t2 t3 => .conv_congr (cvapply σ t1) (cvapply σ t2) (cvapply σ t3)
+    | σ, .conv_erased t => .conv_erased (cvapply σ t)
+
+    @[simp]
+    def apply : Subst Term -> Term -> Term
     | σ, bound c k =>
       match σ k with
       | .replace t => t
@@ -77,9 +155,14 @@ namespace Term
     | σ, subst t1 t2 => subst (apply σ t1) (apply σ t2)
     | σ, phi t1 t2 t3 => phi (apply σ t1) (apply σ t2) (apply σ t3)
     | σ, eq t1 t2 t3 => eq (apply σ t1) (apply σ t2) (apply σ t3)
-    | σ, conv t1 t2 c => conv (apply σ t1) (apply σ t2) c
+    | σ, conv t1 t2 c => conv (apply σ t1) (apply σ t2) (cvapply ▸σ c)
 
-    def compose : Subst -> Subst -> Subst
+    def cvcompose : Subst CvTerm -> Subst CvTerm -> Subst CvTerm
+    | σ, τ, n => match (σ n) with
+      | .replace t => .replace (cvapply τ t)
+      | .rename k => τ k
+
+    def compose : Subst Term -> Subst Term -> Subst Term
     | σ, τ, n => match (σ n) with
       | .replace t => .replace (apply τ t)
       | .rename k => τ k
@@ -89,21 +172,28 @@ namespace Term
   end Subst
 
   -- notation:100 "r#" σ:110 => Subst.from_ren σ
-  prefix:max "r#" => Subst.from_ren
+  prefix:max "r#" => @Subst.from_ren Term
+  prefix:max "cr#" => @Subst.from_ren CvTerm
   -- notation:70 t:70 "::" σ:70 => Subst.cons t σ
   infix:70 "::" => Subst.cons
   --notation:100 "^" σ:110 => Subst.lift σ
   prefix:max "^" => Subst.lift
+  prefix:max "^" => Subst.cvlift
   notation:90 "[" σ "]" t:89 => Subst.apply σ t
+  notation:90 "[" σ "]" t:89 => Subst.cvapply σ t
   notation:90 τ:90 " ⊙ " σ:91 => Subst.compose σ τ
+  notation:90 τ:90 " ⊙ " σ:91 => Subst.cvcompose σ τ
   notation:90 s:90 "β[" t "]" => Subst.beta s t
 
   @[simp] theorem subst_from_ren_x : (r#r) x = .rename (r x) :=
     by unfold Subst.from_ren; rfl
 
-  @[simp] theorem subst_cons_zero (σ : Subst) : (s :: σ) 0 = s :=
+  @[simp] theorem subst_from_cvren_x : (cr#r) x = .rename (r x) :=
+    by unfold Subst.from_ren; rfl
+
+  @[simp] theorem subst_cons_zero (σ : Subst T) : (s :: σ) 0 = s :=
     by unfold Subst.cons; rfl
-  @[simp] theorem subst_cons_succ (σ : Subst) : (s :: σ) (n + 1) = σ n :=
+  @[simp] theorem subst_cons_succ (σ : Subst T) : (s :: σ) (n + 1) = σ n :=
     by unfold Subst.cons; rfl
 
   @[simp]
@@ -123,9 +213,55 @@ namespace Term
   }
 
   @[simp]
+  theorem subst_cvlift_is_ren_cvlift r : cr#(Ren.lift r) = ^(cr#r) := by {
+    funext; case _ x =>
+    cases x
+    case zero =>
+      unfold Subst.from_ren; unfold Ren.lift; simp
+      unfold Subst.cvlift; simp
+    case _ n =>
+      generalize lhsdef : (r#(Ren.lift r)) (n + 1) = lhs
+      generalize rhsdef : (^(r#r)) (n + 1) = rhs
+      unfold Subst.from_ren at lhsdef; simp at *
+      unfold Ren.lift at lhsdef; simp at *
+      unfold Subst.lift at rhsdef; simp at *
+      subst lhsdef; subst rhsdef; rfl
+  }
+
+  @[simp]
+  theorem subst_cvapply_is_ren_cvapply r t : Ren.cvapply r t = [cr#r]t := by {
+    induction t generalizing r
+    any_goals (unfold Ren.cvapply; simp [*])
+  }
+
+  @[simp]
+  theorem subst_from_ren_transport_is_same : ▸(r#r) = cr#r := by {
+    funext
+    case _ x =>
+      cases x
+      all_goals (unfold Subst.from_ren; unfold subst_term_to_subst_cvterm; simp [*])
+  }
+
+  @[simp]
   theorem subst_apply_is_ren_apply r t : Ren.apply r t = [r#r]t := by {
     induction t generalizing r
     any_goals (unfold Ren.apply; simp [*])
+  }
+
+  @[simp]
+  theorem subst_cvapply_I_is_id s : [cr#I]s = s := by {
+    have lem : ^(cr# I) = cr# I := by {
+      funext
+      case _ x =>
+      cases x
+      case _ =>
+        unfold Subst.cvlift; simp
+      case _ x =>
+        unfold Subst.cvlift; simp
+    }
+    induction s
+    all_goals unfold Subst.cvapply
+    any_goals simp [*]
   }
 
   @[simp]
@@ -144,15 +280,161 @@ namespace Term
     any_goals simp [*]
   }
 
+  theorem subst_transform_ren_apply_commutes : cvrefl ([r#r]t) = [cr#r] (cvrefl t) := by {
+    induction t generalizing r
+    all_goals simp [*]
+    case lam m t1 t2 ih1 ih2 => rw [<-subst_cvlift_is_ren_cvlift, <-subst_lift_is_ren_lift, ih2]
+    case all m t1 t2 ih1 ih2 => rw [<-subst_cvlift_is_ren_cvlift, <-subst_lift_is_ren_lift, ih2]
+    case prod t1 t2 ih1 ih2 => rw [<-subst_cvlift_is_ren_cvlift, <-subst_lift_is_ren_lift, ih2]
+  }
+
   @[simp]
-  theorem subst_apply_twice_is_apply_compose s σ τ : [τ][σ]s = [τ ⊙ σ]s := by {
+  theorem subst_transform_lift_commutes : ▸^σ = ^▸σ := by {
+    funext
+    case _ x =>
+    unfold subst_term_to_subst_cvterm; unfold Subst.lift; unfold Subst.cvlift; simp
+    cases x
+    case _ => simp
+    case _ n =>
+      simp
+      cases σ n
+      case _ => simp
+      case _ t =>
+        simp; rw [subst_transform_ren_apply_commutes]
+  }
+
+  theorem subst_transform_apply_commutes : cvrefl ([σ]t) = [▸σ](cvrefl t) := by {
+    induction t generalizing σ
+    all_goals simp [*]
+    case bound k i =>
+      unfold subst_term_to_subst_cvterm; simp
+      cases σ i
+      case _ j => simp
+      case _ s => simp
+  }
+
+  @[simp]
+  theorem subst_transform_commutes_with_compose : ▸(σ ⊙ τ) = ▸σ ⊙ ▸τ := by {
+    funext
+    case _ x =>
+    unfold subst_term_to_subst_cvterm; unfold Subst.compose; unfold Subst.cvcompose; simp
+    cases (τ x)
+    case _ x => simp
+    case _ t =>
+      simp; rw [subst_transform_apply_commutes]
+      unfold subst_term_to_subst_cvterm; simp
+  }
+
+  @[simp]
+  theorem subst_cvapply_twice_is_cvapply_compose {s : CvTerm} {σ τ} : [τ][σ]s = [τ ⊙ σ]s := by {
+    have lem1 τ : ^τ ⊙ cr#S = cr#S ⊙ τ := by {
+      funext
+      unfold Subst.cvcompose; unfold Subst.from_ren; unfold S; simp
+      unfold Subst.cvlift; unfold S; simp
+      unfold Subst.from_ren; simp
+    }
+    have lem2 (σ:Subst CvTerm) e : ^(σ ⊙ cr#e) = ^σ ⊙ ^(cr#e) := by {
+      funext; case _ n =>
+      cases n
+      . unfold Subst.from_ren; unfold Subst.cvcompose; unfold Subst.cvlift; simp
+      case _ n =>
+        generalize lhsdef : (^σ ⊙ ^(cr#e)) (n + 1) = lhs
+        unfold Subst.cvlift; simp
+        unfold Subst.cvcompose; unfold Subst.from_ren; unfold S; simp
+        subst lhs; unfold Subst.cvcompose; unfold Subst.cvlift; simp
+        unfold Subst.from_ren; unfold S; simp
+    }
+    have lem3 σ e s : [σ][cr#e]s = [σ ⊙ cr#e]s := by {
+      induction s generalizing σ e
+      any_goals simp [*]
+      case bound => unfold Subst.cvcompose; simp
+      case all_congr _ _ _ ih => rw [<-subst_cvlift_is_ren_cvlift, ih]
+      case lam_congr _ _ _ ih => rw [<-subst_cvlift_is_ren_cvlift, ih]
+      case lam_mf_erased _ ih => rw [<-subst_cvlift_is_ren_cvlift, ih]
+      case lam_m0_erased _ ih => rw [<-subst_cvlift_is_ren_cvlift, ih]
+      case prod_congr _ _ _ ih => rw [<-subst_cvlift_is_ren_cvlift, ih]
+    }
+    have lem4 σ τ : σ ⊙ τ ⊙ cr#S = σ ⊙ (τ ⊙ cr#S) := by {
+      funext; case _ x =>
+      cases x
+      any_goals (unfold Subst.cvcompose; unfold Subst.from_ren; unfold S; simp)
+    }
+    have lem5 r1 r2 τ : cr#r1 ⊙ (cr#r2 ⊙ τ) = cr#r1 ⊙ cr#r2 ⊙ τ := by {
+      funext; case _ x =>
+        unfold Subst.cvcompose; simp
+        cases τ x <;> simp at *
+        case _ t =>
+          have lem : [fun x => SubstAction.rename (r1 (r2 x))]t = [cr#r1 ⊙ cr#r2]t := by {
+            unfold Subst.cvcompose; simp
+          }
+          rw [lem, lem3]
+    }
+    have lem6 e τ : ^(cr#e) ⊙ ^τ = ^(cr#e ⊙ τ) := by {
+      funext; case _ n =>
+      cases n
+      . unfold Subst.cvcompose; unfold Subst.cvlift; simp
+      case _ n =>
+        have lem : ((^(cr#e) ⊙ ^τ) ⊙ cr#S) n = (^(cr#e ⊙ τ) ⊙ cr#S) n := by {
+          rw [lem1, lem4, lem1]
+          rw [<-subst_cvlift_is_ren_cvlift, lem5]; simp
+          rw [lem1, lem5]
+        }
+        unfold Subst.cvcompose at lem; unfold S at lem; unfold Subst.from_ren at lem
+        unfold Subst.cvcompose; unfold Subst.from_ren
+        simp at lem; simp [*]
+    }
+    have lem7 τ e s : [cr#e][τ]s = [cr#e ⊙ τ]s := by {
+      induction s generalizing τ e
+      any_goals simp [*]
+      case bound k =>
+        unfold Subst.cvcompose; simp
+        cases τ k <;> simp at *
+      case all_congr _ _ _ ih => rw [<-subst_cvlift_is_ren_cvlift, ih, <-lem6]; simp
+      case lam_congr _ _ _ ih => rw [<-subst_cvlift_is_ren_cvlift, ih, <-lem6]; simp
+      case lam_mf_erased _ ih => rw [<-subst_cvlift_is_ren_cvlift, ih, <-lem6]; simp
+      case lam_m0_erased _ ih => rw [<-subst_cvlift_is_ren_cvlift, ih, <-lem6]; simp
+      case prod_congr _ _ _ ih => rw [<-subst_cvlift_is_ren_cvlift, ih, <-lem6]; simp
+    }
+    have lem8 σ τ : σ ⊙ (cr#S ⊙ τ) = σ ⊙ cr#S ⊙ τ := by {
+      funext; case _ x =>
+        unfold Subst.cvcompose; simp
+        cases τ x <;> simp at *
+        rw [lem3]; unfold Subst.cvcompose; simp
+    }
+    have lem9 σ τ : cr#S ⊙ (σ ⊙ τ) = cr#S ⊙ σ ⊙ τ := by {
+      funext; case _ x =>
+        unfold Subst.cvcompose; simp
+        cases τ x <;> simp at *
+        rw [lem7]; unfold Subst.cvcompose; simp
+    }
+    have lem10 (σ τ : Subst CvTerm) : ^σ ⊙ ^τ = ^(σ ⊙ τ) := by {
+      funext; case _ x =>
+      cases x
+      case _ => unfold Subst.cvcompose; unfold Subst.cvlift; simp
+      case _ n =>
+        have lem : ((^σ ⊙ ^τ) ⊙ cr#S) n = (^(σ ⊙ τ) ⊙ cr#S) n := by {
+          rw [lem1, lem4, lem1, lem8, lem1, lem9]
+        }
+        unfold Subst.cvcompose at lem; unfold S at lem; unfold Subst.from_ren at lem
+        unfold Subst.cvcompose
+        simp at lem; simp [*]
+    }
+    induction s generalizing τ σ
+    any_goals simp [*]
+    case bound k =>
+      unfold Subst.cvcompose; simp
+      cases σ k <;> simp
+  }
+
+  @[simp]
+  theorem subst_apply_twice_is_apply_compose {s : Term} {σ τ} : [τ][σ]s = [τ ⊙ σ]s := by {
     have lem1 τ : ^τ ⊙ r#S = r#S ⊙ τ := by {
       funext
       unfold Subst.compose; unfold Subst.from_ren; unfold S; simp
       unfold Subst.lift; unfold S; simp
       unfold Subst.from_ren; simp
     }
-    have lem2 (σ:Subst) e : ^(σ ⊙ r#e) = ^σ ⊙ ^(r#e) := by {
+    have lem2 (σ:Subst Term) e : ^(σ ⊙ r#e) = ^σ ⊙ ^(r#e) := by {
       funext; case _ n =>
       cases n
       . unfold Subst.from_ren; unfold Subst.compose; unfold Subst.lift; simp
@@ -222,7 +504,7 @@ namespace Term
         cases τ x <;> simp at *
         rw [lem7]; unfold Subst.compose; simp
     }
-    have lem10 σ τ : ^σ ⊙ ^τ = ^(σ ⊙ τ) := by {
+    have lem10 (σ τ : Subst Term) : ^σ ⊙ ^τ = ^(σ ⊙ τ) := by {
       funext; case _ x =>
       cases x
       case _ => unfold Subst.compose; unfold Subst.lift; simp
@@ -254,11 +536,31 @@ namespace Term
     : [.rename k :: σ]bound c 0 = bound c k
   := by unfold Subst.cons; simp
 
+  @[simp]
+  theorem cvsubst_valid2_replace
+    : [.replace s :: σ]CvTerm.bound 0 = s
+  := by unfold Subst.cons; simp
+
+  @[simp]
+  theorem cvsubst_valid2_rename
+    : [.rename k :: σ]CvTerm.bound 0 = CvTerm.bound k
+  := by unfold Subst.cons; simp
+
   @[simp] -- ⇑σ = 0.(σ ◦ S)
-  theorem subst_valid3 : ^σ = .rename 0 :: (r#S ⊙ σ) := by {
+  theorem subst_valid3 {σ : Subst Term} : ^σ = .rename 0 :: (r#S ⊙ σ) := by {
     funext; case _ x =>
       unfold Subst.lift; simp
       unfold Subst.compose; simp
+      cases x
+      case _ => simp
+      case _ n => simp
+  }
+
+  @[simp]
+  theorem cvsubst_valid3 {σ : Subst CvTerm} : ^σ = .rename 0 :: (cr#S ⊙ σ) := by {
+    funext; case _ x =>
+      unfold Subst.cvlift; simp
+      unfold Subst.cvcompose; simp
       cases x
       case _ => simp
       case _ n => simp
@@ -274,10 +576,26 @@ namespace Term
       unfold Subst.cons; unfold Subst.from_ren; simp
   }
 
+  @[simp]
+  theorem cvsubst_valid4 : .rename 0 :: cr#S = cr#I := by {
+    funext; case _ x =>
+    cases x
+    case _ =>
+      unfold Subst.cons; unfold Subst.from_ren; simp
+    case _ n =>
+      unfold Subst.cons; unfold Subst.from_ren; simp
+  }
+
   @[simp] -- σ ◦ I = σ
   theorem subst_valid5 : σ ⊙ r#I = σ := by {
     funext; case _ x =>
     unfold Subst.compose; unfold Subst.from_ren; unfold I; simp
+  }
+
+  @[simp]
+  theorem cvsubst_valid5 : σ ⊙ cr#I = σ := by {
+    funext; case _ x =>
+    unfold Subst.cvcompose; unfold Subst.from_ren; unfold I; simp
   }
 
   @[simp] -- I ◦ σ = σ
@@ -290,16 +608,34 @@ namespace Term
     case _ _ _ e => rw [e]
   }
 
+  @[simp]
+  theorem cvsubst_valid6 : cr#I ⊙ σ = σ := by {
+    funext; case _ x =>
+    unfold Subst.cvcompose; simp
+    cases x
+    all_goals (split; simp [*])
+    case _ _ _ e => rw [e]
+    case _ _ _ e => rw [e]
+  }
+
   @[simp] -- (σ ◦ τ) ◦ μ = σ ◦ (τ ◦ μ)
-  theorem subst_valid7 : σ ⊙ (τ ⊙ μ) = σ ⊙ τ ⊙ μ := by {
+  theorem subst_valid7 {σ : Subst Term} : σ ⊙ (τ ⊙ μ) = σ ⊙ τ ⊙ μ := by {
     funext; case _ x =>
       unfold Subst.compose; simp
       cases μ x <;> simp
       . unfold Subst.compose; simp
   }
 
+  @[simp]
+  theorem cvsubst_valid7 {σ : Subst CvTerm} : σ ⊙ (τ ⊙ μ) = σ ⊙ τ ⊙ μ := by {
+    funext; case _ x =>
+      unfold Subst.cvcompose; simp
+      cases μ x <;> simp
+      . unfold Subst.cvcompose; simp
+  }
+
   @[simp] -- (s.σ ) ◦ τ = s[τ].(σ ◦ τ)
-  theorem subst_valid8_replace
+  theorem subst_valid8_replace {s : Term}
     : τ ⊙ (.replace s :: σ) = .replace ([τ]s) :: (τ ⊙ σ)
   := by {
     funext; case _ x =>
@@ -307,13 +643,31 @@ namespace Term
     all_goals (unfold Subst.compose; unfold Subst.cons; simp)
   }
 
+  @[simp]
+  theorem cvsubst_valid8_replace {s : CvTerm}
+    : τ ⊙ (.replace s :: σ) = .replace ([τ]s) :: (τ ⊙ σ)
+  := by {
+    funext; case _ x =>
+    cases x
+    all_goals (unfold Subst.cvcompose; unfold Subst.cons; simp)
+  }
+
   @[simp] -- (s.σ ) ◦ τ = s[τ].(σ ◦ τ)
-  theorem subst_valid8_rename
+  theorem subst_valid8_rename {σ : Subst Term}
     : τ ⊙ (.rename s :: σ) = (τ s) :: (τ ⊙ σ)
   := by {
     funext; case _ x =>
     cases x
     all_goals (unfold Subst.compose; unfold Subst.cons; simp)
+  }
+
+  @[simp] -- (s.σ ) ◦ τ = s[τ].(σ ◦ τ)
+  theorem cvsubst_valid8_rename {σ : Subst CvTerm}
+    : τ ⊙ (.rename s :: σ) = (τ s) :: (τ ⊙ σ)
+  := by {
+    funext; case _ x =>
+    cases x
+    all_goals (unfold Subst.cvcompose; unfold Subst.cons; simp)
   }
 
   @[simp] -- S ◦ (s.σ ) = σ
@@ -322,6 +676,16 @@ namespace Term
     cases x
     all_goals {
       unfold Subst.compose; unfold Subst.cons; unfold Subst.from_ren
+      unfold S; simp
+    }
+  }
+
+  @[simp]
+  theorem cvsubst_valid9 : (s :: σ) ⊙ cr#S = σ := by {
+    funext; case _ x =>
+    cases x
+    all_goals {
+      unfold Subst.cvcompose; unfold Subst.cons; unfold Subst.from_ren
       unfold S; simp
     }
   }
@@ -349,6 +713,13 @@ namespace Term
   theorem subst_rw_ex2 : [t::r#I][^σ]s = [t::σ]s := by simp
   -- s[⇑σ ][t[σ ].I] = s[t.I][σ ]
   theorem subst_rw_ex3 : [(.replace ([σ]t))::r#I][^σ]s = [σ][.replace t::r#I]s := by simp
+
+  -- s[σ ][S] = s[S][⇑σ ]
+  theorem cvsubst_rw_ex1 : [cr#S][σ]s = [^σ][cr#S]s := by simp
+  -- -- s[⇑σ ][t.I] = s[t.σ ]
+  theorem cvsubst_rw_ex2 : [t::cr#I][^σ]s = [t::σ]s := by simp
+  -- s[⇑σ ][t[σ ].I] = s[t.I][σ ]
+  theorem cvsubst_rw_ex3 : [(.replace ([σ]t))::cr#I][^σ]s = [σ][.replace t::cr#I]s := by simp
 
   def mode_to_sort : Mode -> Const
   | mt => .kind
