Common.lean
@@ -1,10 +1,6 @@
 
-import Common.Map
 import Common.Mathlib
-import Common.Name
-import Common.Notation
 import Common.Term
 import Common.Term.Normal
 import Common.Term.Classify
-import Common.Context
 import Common.Util
